theories/L2_5_box/program.v
@@ -38,46 +38,496 @@ Proof.
 Qed.
 
 
-(********
-(** Check that a Term is Canonical (constructor in head)
-*** and return the constructor number and its argument list:
-*** used for a Case step, as the match argument must be canonical
-*** before Case can be evaluated
-**)
-Inductive Canonical : Term -> nat -> Terms -> Prop :=
-| canC: forall (i:inductive) (n:nat),
-          Canonical (TConstruct i n) n tnil
-| canA: forall (i:inductive) (n:nat) (t:Term) (ts:Terms),
-          Canonical (TApp (TConstruct i n) t ts) n (tcons t ts).
-Hint Constructors Canonical.
-
-
-Lemma Canonical_dec:
-  forall t n ts, Canonical t n ts \/ ~ Canonical t n ts.
-induction t; intros; try (solve [right; intros h; inversion_Clear h]).
-- destruct (isConstruct_dec t1). destruct H. elim H. intros.
-  subst. destruct (eq_nat_dec x0 n). subst.
-
-Definition canonical (t:Term) : option (nat * Terms) :=
-  match t with
-    | TConstruct _ n => Some (n, tnil)
-    | TApp (TConstruct _ n) t ts => Some (n, (tcons t ts))
-    | _ => None
-  end.
-
-Lemma Canonical_canonical:
-  forall m t, WFTrm t m -> 
-              forall n ts, Canonical t n ts <-> canonical t = Some (n, ts).
-induction 1; intros xn xts; split; intros h;
-try discriminate; try (inversion h); try reflexivity.
-- destruct fn; try discriminate. injection H4. intros. subst. apply canA.
-- apply canC.
-Qed.
-***)
-
 (** correctness specification for programs (including local closure) **)
+Inductive crctTerm: environ Term -> nat -> Term -> Prop :=
+| ctRel: forall p n m, crctEnv p -> m < n -> crctTerm p n (TRel m)
+| ctCast: forall p n t, crctEnv p -> crctTerm p n t ->
+                        crctTerm p n (TCast t)
+| ctProof: forall p n, crctEnv p -> crctTerm p n TProof
+| ctLam: forall p n nm bod,
+           crctEnv p -> crctTerm p (S n) bod -> crctTerm p n (TLambda nm bod)
+| ctLetIn: forall p n nm dfn bod,
+             crctEnv p -> crctTerm p n dfn -> crctTerm p (S n) bod ->
+             crctTerm p n (TLetIn nm dfn bod)
+| ctApp: forall p n fn arg args,
+           crctEnv p -> crctTerm p n fn -> ~ isApp fn -> crctTerm p n arg ->
+           crctTerms p n args -> crctTerm p n (TApp fn arg args)
+| ctConst: forall p n pd nm,
+             crctEnv p -> LookupDfn nm p pd -> crctTerm p n (TConst nm)
+| ctAx: forall p n, crctEnv p -> crctTerm p n TAx
+| ctConstructor: forall p n ipkgNm inum cnum args ipkg itp cstr pars,
+                   crctEnv p -> LookupTyp ipkgNm p pars ipkg ->
+                   getInd ipkg inum = Ret itp ->
+                   getCnstr itp cnum = Ret cstr ->
+                   crctTerms p n args ->
+                   crctTerm p n (TConstruct (mkInd ipkgNm inum) cnum args)
+| ctCase: forall p n m mch brs,
+            crctEnv p -> crctTerm p n mch -> crctDs p n brs ->
+            crctTerm p n (TCase m mch brs)
+| ctFix: forall p n ds m,
+           crctEnv p -> crctDs p (n + dlength ds) ds -> m < dlength ds ->
+           crctTerm p n (TFix ds m)
+(* crctEnvs are closed in both ways *)
+with crctEnv: environ Term -> Prop :=
+| ceNil: crctEnv nil
+| ceTrmCons: forall nm s p,
+               crctEnv p -> fresh nm p -> crctTerm p 0 s ->
+               crctEnv ((nm,ecTrm s)::p)
+| ceTypCons: forall nm m s p,
+               crctEnv p -> fresh nm p ->
+               crctEnv ((nm,AstCommon.ecTyp Term m s)::p)
+with crctTerms: environ Term -> nat -> Terms -> Prop :=
+| ctsNil: forall p n, crctEnv p -> crctTerms p n tnil
+| ctsCons: forall p n t ts,
+             crctEnv p -> crctTerm p n t -> crctTerms p n ts ->
+             crctTerms p n (tcons t ts)
+with crctDs: environ Term -> nat -> Defs -> Prop :=
+| cdsNil: forall p n, crctEnv p -> crctDs p n dnil
+| cdsCons: forall p n nm bod ix ds,
+             crctEnv p -> crctTerm p n bod -> crctDs p n ds ->
+             crctDs p n (dcons nm bod ix ds).
+Hint Constructors crctTerm crctTerms crctDs crctEnv.
+Scheme crct_ind' := Minimality for crctTerm Sort Prop
+  with crcts_ind' := Minimality for crctTerms Sort Prop
+  with crctDs_ind' := Minimality for crctDs Sort Prop
+  with crctEnv_ind' := Minimality for crctEnv Sort Prop.
+Combined Scheme crctCrctsCrctDsEnv_ind from
+         crct_ind', crcts_ind', crctDs_ind', crctEnv_ind'.
+
+Lemma Crct_WFTrm:
+  (forall p n t, crctTerm p n t -> WFTrm t n) /\
+  (forall p n ts, crctTerms p n ts -> WFTrms ts n) /\
+  (forall p n (ds:Defs), crctDs p n ds -> WFTrmDs ds n) /\
+  (forall p, crctEnv p -> True).
+apply crctCrctsCrctDsEnv_ind; intros; auto.
+Qed.
+
+Lemma Crct_WFApp:
+  forall p n t, crctTerm p n t -> WFapp t.
+  intros p n t h. eapply WFTrm_WFapp. eapply (proj1 Crct_WFTrm). eassumption.
+Qed.
+
+Lemma Crct_up:
+  (forall p n t, crctTerm p n t -> crctTerm p (S n) t) /\
+  (forall p n ts, crctTerms p n ts -> crctTerms p (S n) ts) /\
+  (forall p n (ds:Defs), crctDs p n ds -> crctDs p (S n) ds) /\
+  (forall p, crctEnv p -> True). 
+Proof.
+  apply crctCrctsCrctDsEnv_ind; intros; try (solve [constructor; assumption]).
+  - apply ctRel; try assumption. omega.
+  - eapply ctConst; eassumption.
+  - eapply ctConstructor; eassumption.
+Qed.
+
+Lemma Crct_UP:
+  forall n p t, crctTerm p n t -> forall m, n <= m -> crctTerm p m t.
+Proof.
+  intros n p t h. induction 1. assumption. apply Crct_up. assumption.
+Qed.
+
+Lemma Crct_Up:
+  forall n p t, crctTerm p 0 t -> crctTerm p n t.
+Proof.
+  intros. eapply Crct_UP. eassumption. omega.
+Qed.
+Hint Resolve Crct_Up Crct_UP.
+
+Lemma Crcts_tnil:
+  forall p n t, crctTerm p n t -> crctTerms p 0 tnil.
+Proof.
+  induction 1; apply ctsNil; try assumption;
+  try (solve [eapply Crct_Sort; eassumption]).
+Qed.
+
+Lemma Crct_fresh_Pocc:
+  (forall p n t, crctTerm p n t -> forall nm, fresh nm p -> ~ PoccTrm nm t) /\
+  (forall p n ts, crctTerms p n ts ->
+                  forall nm, fresh nm p -> ~ PoccTrms nm ts) /\
+  (forall p n (ds:Defs), crctDs p n ds ->
+                         forall nm, fresh nm p -> ~ PoccDefs nm ds) /\
+  (forall (p:environ Term), crctEnv p -> True).
+Proof.
+  apply crctCrctsCrctDsEnv_ind; intros; try intros j; auto;
+  inversion_Clear j;
+  try (specialize (H2 _ H3); contradiction);
+  try (specialize (H2 _ H5); contradiction);
+  try (specialize (H4 _ H5); contradiction);
+  try (specialize (H2 _ H8); contradiction);
+  try (specialize (H2 _ H4); contradiction);
+  try (specialize (H5 _ H8); contradiction);
+  try (specialize (H7 _ H8); contradiction).
+  - unfold LookupDfn in H1. elim (Lookup_fresh_neq H1 H2). reflexivity.
+  - unfold LookupTyp in H1. destruct H1.
+    elim (Lookup_fresh_neq H1 H6). reflexivity.
+  - specialize (H5 _ H6). intuition.     
+Qed.
+
+Lemma Crct_weaken:
+  (forall p n t, crctTerm p n t -> 
+                 forall nm s, fresh nm p -> crctTerm p 0 s ->
+                              crctTerm ((nm,ecTrm s)::p) n t) /\
+  (forall p n ts, crctTerms p n ts -> 
+                  forall nm s, fresh nm p -> crctTerm p 0 s ->
+                               crctTerms ((nm,ecTrm s)::p) n ts) /\
+  (forall p n ds, crctDs p n ds -> 
+                  forall nm s, fresh nm p -> crctTerm p 0 s ->
+                               crctDs ((nm,ecTrm s)::p) n ds) /\
+  (forall p, crctEnv p -> True).
+Proof.
+  apply crctCrctsCrctDsEnv_ind; intros;
+  try (solve[repeat econstructor; intuition]);
+  try (econstructor; intuition); try eassumption.
+  - unfold LookupDfn in *. constructor.
+    apply neq_sym. apply (Lookup_fresh_neq H1 H2). eassumption.
+  - destruct H1. unfold LookupTyp. split; try eassumption.
+    constructor; try eassumption.
+    apply neq_sym. apply (Lookup_fresh_neq l). assumption.
+Qed.
+
+Lemma Crct_weaken_Typ:
+  (forall p n t, crctTerm p n t -> 
+                 forall nm s m, fresh nm p ->
+                              crctTerm ((nm,ecTyp Term m s)::p) n t) /\
+  (forall p n ts, crctTerms p n ts -> 
+                  forall nm s m, fresh nm p ->
+                               crctTerms ((nm,ecTyp Term m s)::p) n ts) /\
+  (forall p n ds, crctDs p n ds -> 
+                  forall nm s m, fresh nm p ->
+                               crctDs ((nm,ecTyp Term m s)::p) n ds) /\
+  (forall p, crctEnv p -> True).
+Proof.
+  apply crctCrctsCrctDsEnv_ind; intros;
+  try (solve[repeat econstructor; intuition]);
+  try (econstructor; intuition); try eassumption.
+  - unfold LookupDfn in *. constructor.
+    apply neq_sym. apply (Lookup_fresh_neq H1 H2). eassumption.
+  - destruct H1. unfold LookupTyp. split; try eassumption.
+    constructor; try eassumption.
+    apply neq_sym. apply (Lookup_fresh_neq l). assumption.
+Qed.
+
+Lemma Crct_strengthen:
+  (forall pp n s, crctTerm pp n s -> forall nm ec p, pp = (nm,ec)::p ->
+                 ~ PoccTrm nm s -> crctTerm p n s) /\
+  (forall pp n ss, crctTerms pp n ss -> forall nm ec p, pp = (nm,ec)::p ->
+                 ~ PoccTrms nm ss -> crctTerms p n ss) /\
+  (forall pp n ds, crctDs pp n ds -> forall nm ec p, pp = (nm,ec)::p ->
+                 ~ PoccDefs nm ds -> crctDs p n ds) /\
+  (forall (pp:environ Term), crctEnv pp -> True).
+Proof.
+  apply crctCrctsCrctDsEnv_ind; intros; try (subst p);
+  try (econstructor; eassumption);
+  try (inversion_Clear H; constructor; try assumption;
+       eapply H2; try reflexivity; try eassumption;
+       intros h; elim H4; constructor; assumption).
+  - inversion_Clear H; constructor; try assumption;
+    try (eapply H2; try reflexivity; intros h; elim H6;
+         constructor; assumption);
+    try (eapply H4; try reflexivity; intros h; elim H6;
+         constructor; assumption).
+  - inversion_Clear H; constructor; try assumption;
+    try (eapply H2; try reflexivity; intros h; elim H9;
+         constructor; assumption);
+    try (eapply H5; try reflexivity; intros h; elim H9;
+         constructor; assumption);
+    try (eapply H7; try reflexivity; intros h; elim H9;
+         constructor; assumption).
+  - unfold LookupDfn in *.
+    destruct (string_dec nm nm0).
+    + subst. elim H3. constructor.
+    + inversion_Clear H; econstructor; try assumption; unfold LookupDfn;
+      eapply Lookup_strengthen; try reflexivity; try eassumption.
+  - unfold LookupTyp in *. destruct (string_dec ipkgNm nm).
+    + subst. elim H7. constructor.
+    + destruct H1. pose proof (Lookup_strengthen H1 eq_refl n0) as j.
+      econstructor; try eassumption.
+      * inversion_Clear H; assumption.
+      * unfold LookupTyp. intuition. eassumption.
+      * eapply H5. reflexivity. intros h. elim H7.
+        apply PoCnstrargs. assumption.
+  - inversion_Clear H; econstructor; try assumption;
+    try (eapply H2; try reflexivity; intros h; elim H6;
+         constructor; assumption);
+    try (eapply H4; try reflexivity; intros h; elim H6;
+         constructor; assumption).
+  - inversion_Clear H; econstructor; try assumption;
+    eapply H2; try reflexivity; intros h; elim H5;
+         constructor; assumption.
+  - inversion_Clear H; econstructor; try assumption;
+    try (eapply H2; try reflexivity; intros h; elim H6;
+         constructor; assumption);
+    try (eapply H4; try reflexivity; intros h; elim H6;
+         constructor; assumption).
+  - inversion_Clear H; econstructor; try assumption;
+    try (eapply H2; try reflexivity; intros h; elim H6;
+         constructor; assumption);
+    try (eapply H4; try reflexivity; intros h; elim H6;
+         constructor; assumption).
+Qed.
+
+Lemma TWrong_not_Crct:
+  forall p n, ~ crctTerm p n TWrong.
+Proof.
+  induction p; intros; intros h.
+  - inversion h.
+  - eelim IHp. destruct a. eapply (proj1 Crct_strengthen _ _ _ h).
+    + reflexivity.
+    + intros j. inversion j.
+Qed.
+                                         
+(** Crct inversions **)
+Lemma LookupDfn_pres_Crct:
+  forall p n t, crctTerm p n t ->
+                forall nm u, LookupDfn nm p u -> crctTerm p 0 u.
+Proof.
+  assert (lem:
+            (forall p n t, crctTerm p n t -> 
+                  forall nm u, LookupDfn nm p u -> crctTerm p 0 u) /\
+            (forall p n ts, crctTerms p n ts -> True) /\
+            (forall (p:environ Term) (n:nat) (ds:Defs),
+               crctDs p n ds -> True) /\
+            (forall (p:environ Term), crctEnv p ->
+                         forall nm u, LookupDfn nm p u -> crctTerm p 0 u)).
+  { apply crctCrctsCrctDsEnv_ind; intros; auto; unfold LookupDfn in *;
+    try (eapply H0; eassumption); try (eapply H2; eassumption).
+    - inversion H.
+    - destruct (string_dec nm0 nm).
+      + subst nm0. inversion_Clear H4.
+        eapply Crct_weaken; try assumption. elim H10; reflexivity.
+      + eapply Crct_weaken; try assumption. eapply H0.
+        inversion_Clear H4.
+        * elim n. reflexivity.
+        * eassumption.
+    - destruct (string_dec nm0 nm).
+      + subst nm0. inversion_Clear H2. elim H8. reflexivity.
+      + pose proof (Lookup_strengthen H2 eq_refl n) as j.
+        specialize (H0 _ _ j). eapply Crct_weaken_Typ; try assumption.
+  }
+  apply (proj1 lem).
+Qed.
+
+
+Lemma Crct_invrt_Rel:
+  forall p n m, crctTerm p n (TRel m) -> m < n.
+Proof.
+  intros. inversion_Clear H. assumption.
+Qed.
+
+Lemma Crct_invrt_WkTrm:
+  forall (ev:environ Term) n t, crctTerm ev n t ->
+  forall nm s p, ev = (nm, ecTrm s)::p -> crctTerm p 0 s.
+Proof.
+  induction 1; intros;
+  subst p; inversion_Clear H; assumption.
+Qed.
+
+Lemma Crct_LookupDfn_Crct:
+  forall p, crctEnv p -> forall nm t, LookupDfn nm p t -> crctTerm p 0 t.
+Proof.
+  unfold LookupDfn. induction 1; intros.
+  - inversion H.
+  - apply Crct_weaken; inversion_Clear H2; try assumption.
+    eapply IHcrctEnv. eassumption.
+  - eapply (Crct_weaken_Typ); try assumption. eapply IHcrctEnv.
+    destruct (string_dec nm0 nm).
+    + subst nm. inversion_Clear H1. elim H7. reflexivity.
+    + eapply (Lookup_strengthen H1). reflexivity. assumption.
+Qed.
+      
+Lemma Crct_invrt_Const:
+  forall p n const, crctTerm p n const ->
+  forall nm, const = TConst nm ->
+       exists pd, (LookupDfn nm p pd /\ crctTerm p 0 pd).
+Proof.
+  induction 1; intros; try discriminate. myInjection H1. 
+  pose proof (Crct_LookupDfn_Crct H H0). exists pd. intuition.
+Qed.
+
+Lemma Crct_invrt_Lam:
+  forall p n nm bod, crctTerm p n (TLambda nm bod) -> crctTerm p (S n) bod.
+Proof.
+  intros. inversion_Clear H. assumption.
+Qed.
+
+Lemma Crct_invrt_LetIn:
+  forall p n nm dfn bod, crctTerm p n (TLetIn nm dfn bod) ->
+     crctTerm p n dfn /\ crctTerm p (S n) bod.
+Proof.
+   intros. inversion_Clear H. intuition.
+Qed.
+
+Lemma Crct_invrt_App:
+  forall p n fn arg args,
+    crctTerm p n (TApp fn arg args) ->
+    crctTerm p n fn /\ crctTerm p n arg /\ crctTerms p n args /\ ~(isApp fn).
+Proof.
+   intros. inversion_Clear H. intuition.
+Qed.
+
+Lemma Crct_invrt_Case:
+  forall p n m s us,
+    crctTerm p n (TCase m s us) -> crctTerm p n s /\ crctDs p n us.
+Proof.
+   intros. inversion_Clear H. intuition.
+Qed.
+
+Lemma Crct_invrt_Cast:
+  forall p n t, crctTerm p n (TCast t) -> crctTerm p n t.
+Proof.
+   intros. inversion_Clear H. intuition.
+Qed.
+
+Lemma Crct_invrt_Fix:
+  forall p n ds m, crctTerm p n (TFix ds m) ->
+                   crctDs p (n + dlength ds) ds.
+Proof.
+   intros. inversion_Clear H. intuition.
+Qed.
+
+Lemma Crct_invrt_Construct:
+  forall p n ipkgNm inum cnum arty,
+    crctTerm p n (TConstruct (mkInd ipkgNm inum) cnum arty) ->
+    exists npars itypk,
+      LookupTyp ipkgNm p npars itypk /\
+      exists (ip:ityp), getInd itypk inum = Ret ip /\
+                        exists (ctr:Cnstr), getCnstr ip cnum = Ret ctr.
+Proof.
+  intros. inversion_Clear H. exists pars, ipkg. intuition.
+  exists itp. intuition. exists cstr. intuition.
+Qed.
+
+Lemma Crct_invrt_any:
+  forall p n t, crctTerm p n t -> crctEnv p.
+Proof.
+  intros. inversion_Clear H; assumption.
+Qed.
+
+Lemma CrctDs_invrt:
+  forall n p dts, crctDs p n dts -> 
+    forall m x ix, dnthBody m dts = Some (x, ix) -> crctTerm p n x.
+Proof.
+  induction 1; intros.
+  - cbn in H0. discriminate.
+  - destruct m.
+    + cbn in H2. myInjection H2. assumption.
+    + eapply IHcrctDs. cbn in H2. eassumption.
+Qed.
+
+Lemma Crcts_append:
+  forall p n ts, crctTerms p n ts ->
+  forall us, crctTerms p n us -> crctTerms p n (tappend ts us).
+Proof.
+  induction 1; intros us h; simpl.
+  - assumption.
+  - constructor; intuition.
+Qed.
+
+Lemma mkApp_pres_Crct:
+  forall fn p n, crctTerm p n fn ->
+  forall args, crctTerms p n args -> crctTerm p n (mkApp fn args).
+Proof.
+  induction fn; unfold mkApp; simpl; intros p' nx h0 args h1;
+  destruct args; try assumption;
+  try (solve [inversion_Clear h1; apply ctApp; try assumption; not_isApp]).
+  - destruct (Crct_invrt_App h0) as [j1 [j2 [j3 j4]]].
+    rewrite tappend_tnil. assumption.
+  - destruct (Crct_invrt_App h0) as [j1 [j2 [j3 j4]]].
+    apply ctApp; try assumption. destruct t; simpl.
+    + inversion h1; assumption.
+    + inversion h1. assumption.
+    + apply Crcts_append; assumption.
+Qed.
+
+Lemma Instantiate_pres_Crct:
+  forall tin, 
+    (forall n bod ins,
+       Instantiate tin n bod ins ->
+       forall m p, n <= m -> crctTerm p (S m) bod -> crctTerm p m tin ->
+                   crctTerm p m ins) /\
+    (forall n bods inss,
+       Instantiates tin n bods inss ->
+       forall m p, n <= m -> crctTerms p (S m) bods -> crctTerm p m tin ->
+                   crctTerms p m inss) /\
+    (forall n ds ids,
+       InstantiateDefs tin n ds ids ->
+       forall m p, n <= m -> crctDs p (S m) ds -> crctTerm p m tin ->
+                   crctDs p m ids).
+Proof.
+  intros tin.
+  apply InstInstsDefs_ind; intros; trivial;
+  try (inversion_Clear H0; econstructor; eassumption);
+  try (inversion_Clear H1; constructor; try assumption; apply H; assumption).
+  - inversion_Clear H0. constructor. assumption. omega.
+  - apply ctRel.
+    + inversion H0. assumption.
+    + inversion H0. omega.
+  - inversion_Clear H1. apply H; try assumption.
+  - inversion_Clear H1. constructor; try assumption.
+    apply H; try assumption. omega. apply (proj1 Crct_up). assumption.
+  - inversion_Clear H2. constructor. assumption.
+    + apply H; assumption.
+    + apply H0. omega. assumption. apply (proj1 Crct_up). assumption.
+  - inversion_Clear H3. apply mkApp_pres_Crct.
+    + apply H; assumption.
+    + apply ctsCons; try assumption; intuition.
+  - inversion_Clear H1. econstructor; try eassumption.
+    apply H; try eassumption.
+  - inversion_Clear H2. constructor; try assumption.
+    + apply H; try eassumption.
+    + apply H0; try eassumption.
+  - pose proof (InstantiateDefs_pres_dlength i) as k.
+    inversion_Clear H1. inversion_Clear H8.
+    + inversion H9.
+    + cbn in *. constructor; try assumption; rewrite k in *; try assumption.
+      apply H; try omega.
+      * constructor; try assumption.
+      * eapply Crct_UP. eassumption. omega.
+  - inversion_Clear H2. apply ctsCons; intuition.
+  - inversion_Clear H2. constructor; intuition.
+Qed.
+
+Lemma instantiate_pres_Crct:
+  forall p m bod, crctTerm p (S m) bod -> forall tin, crctTerm p m tin -> 
+                  forall n, n <= m ->  crctTerm p m (instantiate tin n bod).
+Proof.
+  intros.
+  apply (proj1 (Instantiate_pres_Crct tin) _ _ _
+               (proj1 (instantiate_Instantiate tin) _ _));
+    try assumption.
+Qed.
+
+Lemma whBetaStep_pres_Crct:
+  forall p n bod, crctTerm p (S n) bod ->
+                  forall a1 args, crctTerm p n a1 -> crctTerms p n args ->
+                                  crctTerm p n (whBetaStep bod a1 args).
+Proof.
+  intros. unfold whBetaStep. apply mkApp_pres_Crct; try assumption.
+  apply instantiate_pres_Crct; try assumption.  omega.
+Qed.
+
+Lemma fold_left_pres_Crct:
+  forall p m (f:Term -> nat -> Term) (ns:list nat) (t:Term),
+    (forall u, crctTerm p m u -> forall n, crctTerm p m (f u n)) ->
+    crctTerm p m t -> crctTerm p m (fold_left f ns t).
+Proof.
+  intros p n f. induction ns; simpl; intros.
+  - assumption.
+  - apply IHns.
+    + intros. apply H. assumption.
+    + apply H. assumption.
+Qed.
+
+
+
+
+
+
+
+
+
+(***********************  old  ************************
+
 Inductive Crct: environ Term -> nat -> Term -> Prop :=
-| CrctSrt: forall n srt, Crct nil n (TSort srt)
 | CrctPrf: forall n, Crct nil n TProof
 | CrctWkTrmTrm: forall n p t s nm, Crct p n t -> Crct p 0 s ->
            fresh nm p -> Crct ((nm,ecTrm s)::p) n t
@@ -86,8 +536,6 @@ Inductive Crct: environ Term -> nat -> Term -> Prop :=
 | CrctRel: forall n m p, m < n -> Crct p 0 prop -> Crct p n (TRel m)
 | CrctCast: forall n p t, Crct p n t -> Crct p n (TCast t)
 | CrctProof: forall n p, Crct p 0 prop -> Crct p n TProof
-| CrctProd: forall n p nm bod,
-              Crct p 0 prop -> Crct p (S n) bod -> Crct p n (TProd nm bod)
 | CrctLam: forall n p nm bod,
              Crct p 0 prop -> Crct p (S n) bod -> Crct p n (TLambda nm bod)
 | CrctLetIn: forall n p nm dfn bod,
@@ -111,7 +559,6 @@ Inductive Crct: environ Term -> nat -> Term -> Prop :=
 | CrctFix: forall n p ds m,
              Crct p 0 prop ->    (** convenient for IH *)
              CrctDs p (n + dlength ds) ds -> Crct p n (TFix ds m)
-| CrctInd: forall n p ind, Crct p n prop -> Crct p n (TInd ind)
 with Crcts: environ Term -> nat -> Terms -> Prop :=
 | CrctsNil: forall n p, Crct p 0 prop -> Crcts p n tnil
 | CrctsCons: forall n p t ts,
@@ -1155,3 +1602,4 @@ Qed.
 
 **********************************)
 ******************************************)
+****************************************)
