theories/L2k_noCnstrParams/L2k.v
@@ -1,0 +1,5 @@
+(** Collect all of L2 together **)
+
+Require Export L2k.compile.
+Require Export L2k.term L2k.program L2k.wcbvEval L2k.wNorm.
+Require Export L2.stripEvalCommute.
