theories/L2k_noCnstrParams/wNorm.v
@@ -1,0 +1,59 @@
+
+Require Import Coq.Lists.List.
+Require Import Coq.Strings.String.
+Require Import Coq.Strings.Ascii.
+Require Import Coq.Arith.EqNat.
+Require Import Coq.Arith.Compare_dec.
+Require Import Coq.omega.Omega.
+Require Import L2k.term.
+Require Import L2k.program.
+Require Import L2k.wcbvEval.
+
+Local Open Scope string_scope.
+Local Open Scope bool.
+Local Open Scope list.
+Local Open Scope program_scope.
+Set Implicit Arguments.
+
+(** Weak typed normal form: normal form of wndEval:
+*** no wndEval steps possible (including no steps in type fields.
+**)
+Section Sec_environ.
+Variable p:environ Term.
+  
+Inductive WNorm: Term -> Prop :=
+| WNLam: forall nm bod, WNorm (TLambda nm bod)
+| WNFix: forall ds br, WNorm (TFix ds br)
+| WNAx: WNorm TAx
+| WNCase: forall mch n brs,
+            WNorm mch -> ~ isCanonical mch ->
+            WNorm (TCase n mch brs)
+| WNConstruct: forall i n arty, WNorm (TConstruct i n arty)
+| WNApp: forall fn t ts,
+           WNorm fn -> WNorm t -> WNorms ts ->
+           ~ (isLambda fn) -> ~ (isFix fn) -> ~ isApp fn ->
+           WNorm (TApp fn t ts)
+| WNAppFix: forall ds m t ts x ix,
+              WNorms (tcons t ts) ->
+              dnthBody m ds = Some (x, ix) ->
+              ix > tlength ts ->  (* too few args to see rec arg *)
+              WNorm (TApp (TFix ds m) t ts)
+with WNorms: Terms -> Prop :=
+| WNtnil: WNorms tnil
+| WNtcons: forall t ts, WNorm t -> WNorms ts -> WNorms (tcons t ts).
+Hint Constructors WNorm WNorm.
+Scheme WNorm_ind' := Induction for WNorm Sort Prop
+      with WNorms_ind' := Induction for WNorms Sort Prop.
+Combined Scheme WNormWNorms_ind from WNorm_ind', WNorms_ind'.
+
+Lemma WNorms_tappendl:
+  forall ts us, WNorms (tappend ts us) -> WNorms ts.
+Proof.
+  induction ts; intros us h.
+  - constructor.
+  - simpl in h. apply WNtcons; inversion_Clear h.
+    + assumption.
+    + eapply IHts. eassumption.
+Qed.
+
+End Sec_environ.
